Hybrid/Semantics/Assignment.lean
@@ -1,0 +1,135 @@
+import Hybrid.Semantics.Satisfaction
+
+namespace Assignment
+
+variable {α : Type u}
+variable [DecidableEq α]
+variable {symbs : Symbols α}
+variable {s : symbs.signature.S}
+
+  lemma variant_refl {g : Assignment M} : g.variant g x := by
+    unfold Assignment.variant
+    aesop
+
+  @[symm]
+  lemma variant_symm {g g' : Assignment M} : g.variant g' x → g'.variant g x := by
+    unfold Assignment.variant
+    aesop
+
+  @[symm]
+  def free_agree_symm {M : Model symbs} {g g' : Assignment M} {φ : FormL symbs sorts} : g.free_agree g' φ → g'.free_agree g φ := by
+    unfold Assignment.free_agree
+    intro h1 s x h2
+    symm
+    apply h1
+    repeat apply_assumption
+
+  /-
+  Given x and y of the same sort, and g, g' and g'' as in the diagram below, we construct h:
+
+          g ----x---- g'
+          |           |
+          |           |
+          y           y
+          |           |
+          |           |
+          h ----x---- g''
+
+  -/
+  def factor_two_step_variant {M : Model symbs} {x y : symbs.svar s} {g g' g'' : Assignment M} (h1 : g'.variant g x) (h2 : g''.variant g' y) :
+    Σ' h : Assignment M, h.variant g y ∧ h.variant g'' x :=
+    ⟨
+      λ {t : symbs.signature.S} (z : symbs.svar t) =>
+        if s_eq_t : s = t then
+          if s_eq_t ▸ z = y then
+            g'' z
+          else g z
+        else g z,
+        ⟨
+          ⟨
+            by  intros z
+                simp
+                intro _ h3
+                subst h3
+                contradiction,
+            by  intro t z h3
+                simp [h3]
+          ⟩,
+          ⟨
+            by  intros t
+                simp
+                intro h3 h4
+                rw [←not_ne_iff, not_not] at h3 h4
+                rw [ne_comm] at h4
+                simp [h2.1 t h4, h1.1 t h3],
+            by  intro t z h3
+                simp [h3]
+                simp [h2.2 z h3, h1.2 z h3]
+          ⟩
+        ⟩
+    ⟩
+
+  /-
+    If x and y have different sorts, the construction above can't be made (try to define h, you'll see it can't
+    be simultaneously a variant of g and a variant of g'').
+
+    But we can refactor g' and g'' by, in essence, reversing their order, while maintaing the same final result:
+  -/
+  def factor_two_step_variant_diff_sorts {M : Model symbs} {x : symbs.svar s} {y : symbs.svar u} {g g' g'' : Assignment M} (h1 : g'.variant g x) (h2 : g''.variant g' y) (hneq_sorts : ¬s = u) :
+    Σ' h' h'' : Assignment M, h'.variant g y ∧ h''.variant h' x ∧ h''.equal g'' :=
+    let h' : Assignment M :=
+      λ {t : symbs.signature.S} (z : symbs.svar t) =>
+        if s_eq_t : t = u then
+          if s_eq_t ▸ z = y then
+            g'' z
+          else g z
+        else g z
+    let h'' :=
+      λ {t : symbs.signature.S} (z : symbs.svar t) =>
+        if s_eq_t : t = s then
+          if s_eq_t ▸ z = x then
+            g' z
+          else h' z
+        else h' z
+    ⟨h', ⟨h'',
+      ⟨by unfold variant h'; aesop,
+      ⟨by unfold variant h'; aesop,
+      by
+        intro t z
+        simp
+        unfold variant at h1 h2
+        have ⟨a, b⟩ := h1
+        have ⟨c, d⟩ := h2
+        clear h1 h2
+        simp only [ne_eq] at a b c d
+        by_cases h_sort : s = t
+        . subst h_sort
+          by_cases h_var : z = x
+          . subst h_var
+            . by_cases h_sort : u = s
+              . subst h_sort
+                contradiction
+              . simp [h'']
+                aesop
+          . simp [h'', h', h_var, hneq_sorts]
+            have sorts_symm : ¬u = s := by intro; apply hneq_sorts; aesop
+            have var_symm : ¬x = z := by intro; apply h_var; aesop
+            specialize d z sorts_symm
+            rw [d]
+            specialize a z var_symm
+            rw [a]
+        . by_cases h_sort : u = t
+          . subst h_sort
+            by_cases h_var : y = z
+            . simp [h'']
+              symm; aesop
+            . simp [h'']
+              symm; aesop
+          . simp [h'']
+            symm; aesop
+        ⟩
+      ⟩
+      ⟩
+    ⟩
+
+end Assignment
